@prefix : <http://bimerr.iot.linkeddata.es/def/occupancy-profile#> .
@prefix dc: <http://purl.org/dc/elements/1.1> .
@prefix op: <http://bimerr.iot.linkeddata.es/def/occupancy-profile#> .
@prefix owl: <http://www.w3.org/2002/07/owl#> .
@prefix rdf: <http://www.w3.org/1999/02/22-rdf-syntax-ns#> .
@prefix xml: <http://www.w3.org/XML/1998/namespace> .
@prefix xsd: <http://www.w3.org/2001/XMLSchema#> .
@prefix foaf: <http://xmlns.com/foaf/0.1#> .
@prefix rdfs: <http://www.w3.org/2000/01/rdf-schema#> .
@prefix time: <http://www.w3.org/2006/time#> .
@prefix vann: <http://purl.org/vocab/vann/> .
@prefix saref: <https://saref.etsi.org/core#> .
@prefix s4bldg: <https://w3id.org/def/saref4building#> .
@prefix dcterms: <http://purl.org/dc/terms/> .
@prefix building: <http://bimerr.iot.linkeddata.es/def/building#> .
@base <http://bimerr.iot.linkeddata.es/def/occupancy-profile#> .

<http://bimerr.iot.linkeddata.es/def/occupancy-profile#> rdf:type owl:Ontology ;
                                                          <http://purl.org/dc/elements/1.1/creator> "María Poveda Villalón" ,
                                                                                                    "Raúl García Castro" ,
                                                                                                    "Serge Chávez Feria" ;
                                                          <http://purl.org/dc/elements/1.1/description> "The Occupancy Profile ontology has been developed to represent and define occupancy profiles in building spaces.|"@en ;
                                                          <http://purl.org/dc/elements/1.1/publisher> "http://www.oeg-upm.net/"@en ;
                                                          <http://purl.org/dc/elements/1.1/title> "Occupancy Profile ontology"@en ;
                                                          dcterms:creator <http://www.oeg-upm.net/> ;
                                                          dcterms:license "http://purl.org/NET/rdflicense/cc-by4.0"@en ;
                                                          vann:preferredNamespacePrefix "op"@en ;
                                                          vann:preferredNamespaceUri "http://bimerr.iot.linkeddata.es/def/occupancy-profile#" ;
                                                          owl:versionInfo "0.1.1" .

#################################################################
#    Annotation properties
#################################################################

###  http://purl.org/dc/elements/1.1/created
<http://purl.org/dc/elements/1.1/created> rdf:type owl:AnnotationProperty .


###  http://purl.org/dc/elements/1.1/creator
<http://purl.org/dc/elements/1.1/creator> rdf:type owl:AnnotationProperty .


###  http://purl.org/dc/elements/1.1/description
<http://purl.org/dc/elements/1.1/description> rdf:type owl:AnnotationProperty .


###  http://purl.org/dc/elements/1.1/publisher
<http://purl.org/dc/elements/1.1/publisher> rdf:type owl:AnnotationProperty .


###  http://purl.org/dc/elements/1.1/title
<http://purl.org/dc/elements/1.1/title> rdf:type owl:AnnotationProperty .


###  http://purl.org/dc/terms/creator
dcterms:creator rdf:type owl:AnnotationProperty .


###  http://purl.org/dc/terms/license
dcterms:license rdf:type owl:AnnotationProperty .


###  http://purl.org/dc/terms/modified
dcterms:modified rdf:type owl:AnnotationProperty .


###  http://purl.org/vocab/vann/preferredNamespacePrefix
vann:preferredNamespacePrefix rdf:type owl:AnnotationProperty .


###  http://purl.org/vocab/vann/preferredNamespaceUri
vann:preferredNamespaceUri rdf:type owl:AnnotationProperty .


#################################################################
#    Datatypes
#################################################################

###  http://www.w3.org/2001/XMLSchema#date
xsd:date rdf:type rdfs:Datatype .


###  http://www.w3.org/2001/XMLSchema#duration
xsd:duration rdf:type rdfs:Datatype .


###  http://www.w3.org/2001/XMLSchema#gMonthDay
xsd:gMonthDay rdf:type rdfs:Datatype .


###  http://www.w3.org/2001/XMLSchema#time
xsd:time rdf:type rdfs:Datatype .


#################################################################
#    Object Properties
#################################################################

###  http://bimerr.iot.linkeddata.es/def/building#hasApartment
building:hasApartment rdf:type owl:ObjectProperty ;
                      rdfs:comment "Relation between a storey and the apartments it is composed of."@en ;
                      rdfs:label "has apartment"@en .


###  http://bimerr.iot.linkeddata.es/def/building#hasSpace
building:hasSpace rdf:type owl:ObjectProperty ;
                  rdfs:comment "Relation to spaces contained in a zone."@en ;
                  rdfs:label "has space"@en .


###  http://bimerr.iot.linkeddata.es/def/occupancy-profile#composedOf
op:composedOf rdf:type owl:ObjectProperty ;
              rdfs:domain op:DriverSet ;
              rdfs:range op:Driver ;
              rdfs:comment "Relationship that indicates the composition of a set of drivers."@en ;
              rdfs:label "composed of"@en .


###  http://bimerr.iot.linkeddata.es/def/occupancy-profile#definedByRange
op:definedByRange rdf:type owl:ObjectProperty ,
                           owl:FunctionalProperty ;
                  rdfs:domain op:PhysicalNeed ;
                  rdfs:range op:ParameterRange ;
                  rdfs:comment "Property used to describe occupant needs by defining comfort limits w.r.t. an environmental parameter."@en ;
                  rdfs:label "defined by range"@en .


###  http://bimerr.iot.linkeddata.es/def/occupancy-profile#describedByFormula
op:describedByFormula rdf:type owl:ObjectProperty ,
                               owl:FunctionalProperty ;
                      rdfs:domain op:Interaction ;
                      rdfs:range op:InteractionFormula ;
                      rdfs:comment "Property to relate an interaction with a formula describing the probability of occurance."@en ;
                      rdfs:label "described by formula"@en .


###  http://bimerr.iot.linkeddata.es/def/occupancy-profile#describesParameter
op:describesParameter rdf:type owl:ObjectProperty ,
                               owl:FunctionalProperty ;
                      rdfs:domain op:ParameterRange ;
                      rdfs:range op:ParameterRange ;
                      rdfs:comment "Relates a comfort envelop with an environmental parameter."@en ;
                      rdfs:label "describes parameter"@en .


###  http://bimerr.iot.linkeddata.es/def/occupancy-profile#detailedBy
op:detailedBy rdf:type owl:ObjectProperty ,
                       owl:FunctionalProperty ;
              rdfs:domain op:Spatial ;
              rdfs:range building:Space ;
              rdfs:comment "Relates a spatial driver to an specific building space"@en ;
              rdfs:label "detailed by"@en .


###  http://bimerr.iot.linkeddata.es/def/occupancy-profile#drivenBy
op:drivenBy rdf:type owl:ObjectProperty ;
            rdfs:domain op:Behavior ;
            rdfs:range op:DriverSet ;
            rdfs:comment "Property to link an occupant with a set of internal or external drivers that are controlling its interactions with building systems."@en ;
            rdfs:label "driven by"@en .


###  http://bimerr.iot.linkeddata.es/def/occupancy-profile#hasBehavior
op:hasBehavior rdf:type owl:ObjectProperty ;
               rdfs:domain op:Occupant ;
               rdfs:range op:Behavior ;
               rdfs:comment "Property to indicate that an occupant has a behavior."@en ;
               rdfs:label "has behavior"@en .


###  http://bimerr.iot.linkeddata.es/def/occupancy-profile#hasCoefficient
op:hasCoefficient rdf:type owl:ObjectProperty ;
                  rdfs:domain op:InteractionFormula ;
                  rdfs:range op:Coefficient ;
                  rdfs:comment "Relates a formula with a coefficient."@en ;
                  rdfs:label "has coefficient"@en .


###  http://bimerr.iot.linkeddata.es/def/occupancy-profile#hasDayOfWeek
op:hasDayOfWeek rdf:type owl:ObjectProperty ,
                         owl:FunctionalProperty ;
                rdfs:domain op:Time ;
                rdfs:range time:DayOfWeek ;
                rdfs:comment "Indicates which days of the week are behavioral drivers for an occupant."@en ;
                rdfs:label "has day of week"@en .


###  http://bimerr.iot.linkeddata.es/def/occupancy-profile#hasEnvironmentalParameter
op:hasEnvironmentalParameter rdf:type owl:ObjectProperty ;
                             rdfs:domain op:Environment ;
                             rdfs:range op:EnvironmentalParameter ;
                             rdfs:comment "Relates and occupant environmental driver with an environmental property like temperature or illuminance."@en ;
                             rdfs:label "has environmental parameter"@en .


###  http://bimerr.iot.linkeddata.es/def/occupancy-profile#hasIndependentVariable
op:hasIndependentVariable rdf:type owl:ObjectProperty ;
                          rdfs:domain op:InteractionFormula ;
                          rdfs:range op:EnvironmentalParameter ;
                          rdfs:comment "Relates a formula with an independent variable."@en ;
                          rdfs:label "has independent variable"@en .


###  http://bimerr.iot.linkeddata.es/def/occupancy-profile#hasMeeting
op:hasMeeting rdf:type owl:ObjectProperty ;
              rdfs:domain building:Space ;
              rdfs:range op:Meeting ;
              rdfs:comment "Indicates that a meeting can occur within a space."@en ;
              rdfs:label "has meeting"@en .


###  http://bimerr.iot.linkeddata.es/def/occupancy-profile#hasOccupant
op:hasOccupant rdf:type owl:ObjectProperty ;
               rdfs:domain building:Space ;
               rdfs:range op:Occupant ;
               rdfs:comment "Relationship that indicates that an space can have an occupant."@en ;
               rdfs:label "has occupant"@en .


###  http://bimerr.iot.linkeddata.es/def/occupancy-profile#hasOperationalMode
op:hasOperationalMode rdf:type owl:ObjectProperty ;
                      rdfs:domain s4bldg:PhysicalObject ;
                      rdfs:range op:OperationalModeConcept ;
                      rdfs:comment "Relationship to indicate the type of control mode of a system, such as fixed or operable modes for a window."@en ;
                      rdfs:label "has operational mode"@en .


###  http://bimerr.iot.linkeddata.es/def/occupancy-profile#hasSeason
op:hasSeason rdf:type owl:ObjectProperty ,
                      owl:FunctionalProperty ;
             rdfs:domain op:Time ;
             rdfs:range op:Season ;
             rdfs:comment "Indicates which seasons are behavioral drivers for an occupant."@en ;
             rdfs:label "has season"@en .


###  http://bimerr.iot.linkeddata.es/def/occupancy-profile#hasTimeOfDay
op:hasTimeOfDay rdf:type owl:ObjectProperty ,
                         owl:FunctionalProperty ;
                rdfs:domain op:Time ;
                rdfs:range op:TimeOfDay ;
                rdfs:comment "Indicates which times during a day are behavioral drivers for an occupant."@en ;
                rdfs:label "has time of day"@en .


###  http://bimerr.iot.linkeddata.es/def/occupancy-profile#hasTransitionType
op:hasTransitionType rdf:type owl:ObjectProperty ;
                     rdfs:domain op:StatusTransition ;
                     rdfs:range op:StatusTransitionTypeConcept ;
                     rdfs:comment "Relationship that indicates the type of status transition event."@en ;
                     rdfs:label "has transition type"@en .


###  http://bimerr.iot.linkeddata.es/def/occupancy-profile#hasUnitOfMeasure
op:hasUnitOfMeasure rdf:type owl:ObjectProperty ,
                             owl:FunctionalProperty ;
                    rdfs:domain op:EnvironmentalParameter ;
                    rdfs:range <https://w3id.org/saref#UnitOfMeasure> ;
                    rdfs:comment "Relates an environmental parameter with a unit of measure."@en ;
                    rdfs:label "has unit of measure"@en .


###  http://bimerr.iot.linkeddata.es/def/occupancy-profile#influencedByNeed
op:influencedByNeed rdf:type owl:ObjectProperty ;
                    rdfs:domain op:Behavior ;
                    rdfs:range op:Need ;
                    rdfs:comment "Indicates that a driver can be influenced by an occupant comfort need."@en ;
                    rdfs:label "influenced by need"@en .


###  http://bimerr.iot.linkeddata.es/def/occupancy-profile#interactsOver
op:interactsOver rdf:type owl:ObjectProperty ,
                          owl:FunctionalProperty ;
                 rdfs:domain op:Interaction ;
                 rdfs:range s4bldg:PhysicalObject ;
                 rdfs:comment "Relationship that describes an interaction between an occupant and a building component or system."@en ;
                 rdfs:label "interacts over"@en .


###  http://bimerr.iot.linkeddata.es/def/occupancy-profile#leadsTo
op:leadsTo rdf:type owl:ObjectProperty ;
           rdfs:domain op:Behavior ;
           rdfs:range op:Action ;
           rdfs:comment "Relationship to indicate the outcome of a behavior. It could lead to an action over a building system to recover comfort or to a passive acceptance of the environmental conditions."@en ;
           rdfs:label "leads to"@en .


###  http://bimerr.iot.linkeddata.es/def/occupancy-profile#relatedToSpace
op:relatedToSpace rdf:type owl:ObjectProperty ;
                  rdfs:domain op:SpaceOccupancy ;
                  rdfs:range building:Space ;
                  rdfs:comment "Property that relates space occupancy events to an specific building space."@en ;
                  rdfs:label "related to space"@en .


###  http://bimerr.iot.linkeddata.es/def/occupancy-profile#specifiedBy
op:specifiedBy rdf:type owl:ObjectProperty ;
               rdfs:domain op:StatusTransition ;
               rdfs:range op:MovementModel ;
               rdfs:comment "Relates a transition event to a movement model that describe this action."@en ;
               rdfs:label "specified by"@en .


###  http://www.w3.org/2004/02/skos/core#broader
<http://www.w3.org/2004/02/skos/core#broader> rdf:type owl:ObjectProperty ;
                                              rdfs:domain <http://www.w3.org/2004/02/skos/core#Concept> ;
                                              rdfs:range <http://www.w3.org/2004/02/skos/core#Concept> ;
                                              rdfs:comment "The property skos:broader is used to assert a direct hierarchical link between two SKOS concepts. A triple <A> skos:broader <B> asserts that <B>, the object of the triple, is a broader concept than <A>, the subject of the triple."@en ;
                                              rdfs:label "broader"@en .


###  http://www.w3.org/2004/02/skos/core#inScheme
<http://www.w3.org/2004/02/skos/core#inScheme> rdf:type owl:ObjectProperty ;
                                               rdfs:domain <http://www.w3.org/2004/02/skos/core#Concept> ;
                                               rdfs:range <http://www.w3.org/2004/02/skos/core#ConceptScheme> ;
                                               rdfs:comment "Property used to indicate that an SKOS concept in within an specific SKOS scheme."@en ;
                                               rdfs:label "in scheme"@en .


###  http://www.w3.org/2004/02/skos/core#narrower
<http://www.w3.org/2004/02/skos/core#narrower> rdf:type owl:ObjectProperty ;
                                               rdfs:domain <http://www.w3.org/2004/02/skos/core#Concept> ;
                                               rdfs:range <http://www.w3.org/2004/02/skos/core#Concept> ;
                                               rdfs:comment "The property skos:narrower is used to assert a direct hierarchical link between two SKOS concepts. A triple <C> skos:narrower <D> asserts that <D>, the object of the triple, is a narrower concept than <C>, the subject of the triple."@en ;
                                               rdfs:label "narrower"@en .


###  https://w3id.org/def/saref4building#contains
s4bldg:contains rdf:type owl:ObjectProperty ;
                rdfs:comment "A relation between a physical space and the objects located in such space."@en ;
                rdfs:label "contains"@en .


#################################################################
#    Data properties
#################################################################

###  http://bimerr.iot.linkeddata.es/def/occupancy-profile#buildingAddress
op:buildingAddress rdf:type owl:DatatypeProperty ;
                   rdfs:range xsd:string ;
                   rdfs:comment "A relationship indicating the address of a building"@en ;
                   rdfs:label "building address"@en .


###  http://bimerr.iot.linkeddata.es/def/occupancy-profile#coefficientValue
op:coefficientValue rdf:type owl:DatatypeProperty ;
                    rdfs:domain op:Coefficient ;
                    rdfs:range xsd:float ;
                    rdfs:comment "A relationship indicating the value of a coefficient."@en ;
                    rdfs:label "coefficient value"@en .


###  http://bimerr.iot.linkeddata.es/def/occupancy-profile#controlValue
op:controlValue rdf:type owl:DatatypeProperty ;
                rdfs:domain op:Interaction ;
                rdfs:range xsd:float ;
                rdfs:comment "A relationship indicating the magnitud of a control action over a building system."@en ;
                rdfs:label "control value"@en .


###  http://bimerr.iot.linkeddata.es/def/occupancy-profile#duration
op:duration rdf:type owl:DatatypeProperty ;
            rdfs:range xsd:duration ;
            rdfs:comment "Average duration of an event."@en ;
            rdfs:label "duration"@en .


###  http://bimerr.iot.linkeddata.es/def/occupancy-profile#earlyOccurTime
op:earlyOccurTime rdf:type owl:DatatypeProperty ;
                  rdfs:range xsd:time ;
                  rdfs:comment "Earliest occurrence time of an event."@en ;
                  rdfs:label "early occur time"@en .


###  http://bimerr.iot.linkeddata.es/def/occupancy-profile#endSeason
op:endSeason rdf:type owl:DatatypeProperty ;
             rdfs:domain op:Season ;
             rdfs:range xsd:gMonthDay ;
             rdfs:comment "Relationship that indicates the month when a season ends."@en ;
             rdfs:label "end season"@en .


###  http://bimerr.iot.linkeddata.es/def/occupancy-profile#endTime
op:endTime rdf:type owl:DatatypeProperty ;
           rdfs:range xsd:dateTime ;
           rdfs:comment "The end time of an event or activity."@en ;
           rdfs:label "end time"@en .


###  http://bimerr.iot.linkeddata.es/def/occupancy-profile#identifier
op:identifier rdf:type owl:DatatypeProperty ,
                       owl:FunctionalProperty ;
              rdfs:comment "Identifier of an element given in the obXML file. Attribute considered for backward compatibility."@en ;
              rdfs:label "identifier"@en .


###  http://bimerr.iot.linkeddata.es/def/occupancy-profile#ifcIdentifier
op:ifcIdentifier rdf:type owl:DatatypeProperty ;
                 rdfs:range xsd:string ;
                 rdfs:comment "Guid of the entity in the IFC file"@en ;
                 rdfs:label "ifc identifier"@en .


###  http://bimerr.iot.linkeddata.es/def/occupancy-profile#maxOccupants
op:maxOccupants rdf:type owl:DatatypeProperty ,
                         owl:FunctionalProperty ;
                rdfs:domain building:Space ;
                rdfs:range xsd:integer ;
                rdfs:comment "Relationship that indicates the maximum number of occupants inside a space."@en ;
                rdfs:label "max number occupants"@en .


###  http://bimerr.iot.linkeddata.es/def/occupancy-profile#maxRangeValue
op:maxRangeValue rdf:type owl:DatatypeProperty ,
                          owl:FunctionalProperty ;
                 rdfs:domain op:ParameterRange ;
                 rdfs:range xsd:float ;
                 rdfs:comment "Upper boundary of a parameter range description."@en ;
                 rdfs:label "max range value"@en .


###  http://bimerr.iot.linkeddata.es/def/occupancy-profile#minOccupants
op:minOccupants rdf:type owl:DatatypeProperty ,
                         owl:FunctionalProperty ;
                rdfs:domain building:Space ;
                rdfs:range xsd:integer ;
                rdfs:comment "Relationship that indicates the minimum number of occupants inside a space."@en ;
                rdfs:label "min number occupants"@en .


###  http://bimerr.iot.linkeddata.es/def/occupancy-profile#minRangeValue
op:minRangeValue rdf:type owl:DatatypeProperty ,
                          owl:FunctionalProperty ;
                 rdfs:domain op:ParameterRange ;
                 rdfs:range xsd:float ;
                 rdfs:comment "Lower boundary of a parameter range description."@en ;
                 rdfs:label "min range value"@en .


###  http://bimerr.iot.linkeddata.es/def/occupancy-profile#occupantAge
op:occupantAge rdf:type owl:DatatypeProperty ,
                        owl:FunctionalProperty ;
               rdfs:domain op:Occupant ;
               rdfs:range xsd:integer ;
               rdfs:comment "Age of an occupant"@en ;
               rdfs:label "occupant age"@en .


###  http://bimerr.iot.linkeddata.es/def/occupancy-profile#occupantGender
op:occupantGender rdf:type owl:DatatypeProperty ,
                           owl:FunctionalProperty ;
                  rdfs:domain op:Occupant ;
                  rdfs:range xsd:string ;
                  rdfs:comment "Gender of an occupant"@en ;
                  rdfs:label "occupant gender"@en .


###  http://bimerr.iot.linkeddata.es/def/occupancy-profile#occupantJobtype
op:occupantJobtype rdf:type owl:DatatypeProperty ,
                            owl:FunctionalProperty ;
                   rdfs:domain op:Occupant ;
                   rdfs:range xsd:string ;
                   rdfs:comment "Jobtype of an occupant"@en ;
                   rdfs:label "occupant jobtype"@en .


###  http://bimerr.iot.linkeddata.es/def/occupancy-profile#occupantLifestyle
op:occupantLifestyle rdf:type owl:DatatypeProperty ,
                              owl:FunctionalProperty ;
                     rdfs:domain op:Occupant ;
                     rdfs:range xsd:string ;
                     rdfs:comment "Lifestyle of an occupant"@en ;
                     rdfs:label "occupant lifestyle"@en .


###  http://bimerr.iot.linkeddata.es/def/occupancy-profile#onHolidays
op:onHolidays rdf:type owl:DatatypeProperty ;
              rdfs:domain op:Time ;
              rdfs:range xsd:date ;
              rdfs:comment "Indicates which days that act as time drivers are holidays."@en ;
              rdfs:label "on holidays"@en .


###  http://bimerr.iot.linkeddata.es/def/occupancy-profile#percentTimePresence
op:percentTimePresence rdf:type owl:DatatypeProperty ;
                       rdfs:domain op:SpaceOccupancy ;
                       rdfs:range xsd:float ;
                       rdfs:comment "Percentage of occupancy time in a space."@en ;
                       rdfs:label "percent time presence"@en .


###  http://bimerr.iot.linkeddata.es/def/occupancy-profile#probability
op:probability rdf:type owl:DatatypeProperty ;
               rdfs:range xsd:float ;
               rdfs:comment "Relationship that links a probility to an event. For example the occurance probability of a meeting."@en ;
               rdfs:label "probability"@en .


###  http://bimerr.iot.linkeddata.es/def/occupancy-profile#startSeason
op:startSeason rdf:type owl:DatatypeProperty ;
               rdfs:domain op:Season ;
               rdfs:range xsd:gMonthDay ;
               rdfs:comment "Relationship that indicates the month when a season start."@en ;
               rdfs:label "start season"@en .


###  http://bimerr.iot.linkeddata.es/def/occupancy-profile#startTime
op:startTime rdf:type owl:DatatypeProperty ;
             rdfs:range xsd:dateTime ;
             rdfs:comment "The start time of an event or activity."@en ;
             rdfs:label "start time"@en .


###  http://bimerr.iot.linkeddata.es/def/occupancy-profile#typicalDuration
op:typicalDuration rdf:type owl:DatatypeProperty ;
                   rdfs:domain op:SpaceOccupancy ;
                   rdfs:range xsd:duration ;
                   rdfs:comment "The typical duration of an event or activity."@en ;
                   rdfs:label "typical duration"@en .


###  http://bimerr.iot.linkeddata.es/def/occupancy-profile#typicalTime
op:typicalTime rdf:type owl:DatatypeProperty ;
               rdfs:range xsd:time ;
               rdfs:comment "Typical occurrence time of an event."@en ;
               rdfs:label "typical time"@en .


#################################################################
#    Classes
#################################################################

###  http://bimerr.iot.linkeddata.es/def/building#Apartment
building:Apartment rdf:type owl:Class ;
                   rdfs:subClassOf [ rdf:type owl:Restriction ;
                                     owl:onProperty building:hasSpace ;
                                     owl:allValuesFrom building:Space
                                   ] ,
                                   [ rdf:type owl:Restriction ;
                                     owl:onProperty op:ifcIdentifier ;
                                     owl:cardinality "1"^^xsd:nonNegativeInteger
                                   ] ;
                   rdfs:comment "An apartment is a group of spaces, partial spaces or other zones."@en ;
                   rdfs:label "Apartment"@en .


###  http://bimerr.iot.linkeddata.es/def/building#Building
building:Building rdf:type owl:Class ;
                  rdfs:subClassOf [ rdf:type owl:Restriction ;
                                    owl:onProperty building:hasApartment ;
                                    owl:allValuesFrom building:Apartment
                                  ] ,
                                  [ rdf:type owl:Restriction ;
                                    owl:onProperty op:ifcIdentifier ;
                                    owl:cardinality "1"^^xsd:nonNegativeInteger
                                  ] ;
                  rdfs:comment "A building represents a structure that provides shelter for its occupants or contents and stands in one place. The building is also used to provide a basic element within the spatial structure hierarchy for the components of a building project (together with site, storey, and space)."@en ;
                  rdfs:label "Building"@en .


###  http://bimerr.iot.linkeddata.es/def/building#Space
building:Space rdf:type owl:Class ;
               rdfs:subClassOf [ rdf:type owl:Restriction ;
                                 owl:onProperty s4bldg:contains ;
                                 owl:someValuesFrom s4bldg:PhysicalObject
                               ] ,
                               [ rdf:type owl:Restriction ;
                                 owl:onProperty op:hasMeeting ;
                                 owl:allValuesFrom op:Meeting
                               ] ,
                               [ rdf:type owl:Restriction ;
                                 owl:onProperty op:hasOccupant ;
                                 owl:allValuesFrom op:Occupant
                               ] ,
                               [ rdf:type owl:Restriction ;
                                 owl:onProperty op:maxOccupants ;
                                 owl:allValuesFrom xsd:integer
                               ] ,
                               [ rdf:type owl:Restriction ;
                                 owl:onProperty op:minOccupants ;
                                 owl:allValuesFrom xsd:integer
                               ] ,
                               [ rdf:type owl:Restriction ;
                                 owl:onProperty op:ifcIdentifier ;
                                 owl:cardinality "1"^^xsd:nonNegativeInteger
                               ] ;
               rdfs:comment "Class to represent the different spaces the building have and where the occupant behaviors occur." ;
               rdfs:label "Space"@en .


###  http://bimerr.iot.linkeddata.es/def/occupancy-profile#AccousticNeed
op:AccousticNeed rdf:type owl:Class ;
                 rdfs:subClassOf op:PhysicalNeed ;
                 rdfs:comment "Range of parameter values where occupants do not feel accoustic discomfort and therefore, they don't carry out any actions."@en ;
                 rdfs:label "Accoustic Need"@en .


###  http://bimerr.iot.linkeddata.es/def/occupancy-profile#Action
op:Action rdf:type owl:Class ;
          rdfs:comment "Actions are the interactions with systems or activities that an occupant can conduct to achieve environmental comfort. Actions connect occupants' inside-world needs with the environmental outside world. (Defintion taken from obXML)"@en ;
          rdfs:label "Action"@en .


###  http://bimerr.iot.linkeddata.es/def/occupancy-profile#Behavior
op:Behavior rdf:type owl:Class ;
            rdfs:subClassOf [ rdf:type owl:Restriction ;
                              owl:onProperty op:drivenBy ;
                              owl:someValuesFrom op:DriverSet
                            ] ,
                            [ rdf:type owl:Restriction ;
                              owl:onProperty op:leadsTo ;
                              owl:someValuesFrom [ rdf:type owl:Class ;
                                                   owl:unionOf ( op:Action
                                                                 op:Inaction
                                                               )
                                                 ]
                            ] ,
                            [ rdf:type owl:Restriction ;
                              owl:onProperty op:influencedByNeed ;
                              owl:allValuesFrom op:Need
                            ] ,
                            [ rdf:type owl:Restriction ;
                              owl:onProperty op:identifier ;
                              owl:someValuesFrom xsd:string
                            ] ;
            rdfs:comment "Behavior related to the interaction with buildings"@en ;
            rdfs:label "Behavior"@en .


###  http://bimerr.iot.linkeddata.es/def/occupancy-profile#Coefficient
op:Coefficient rdf:type owl:Class ;
               rdfs:subClassOf [ rdf:type owl:Restriction ;
                                 owl:onProperty op:coefficientValue ;
                                 owl:someValuesFrom xsd:float
                               ] ;
               rdfs:comment "Class to represent the value and name of coefficients inside mathematical formulas."@en ;
               rdfs:label "Coefficient"@en .


###  http://bimerr.iot.linkeddata.es/def/occupancy-profile#ConstantValueFormula
op:ConstantValueFormula rdf:type owl:Class ;
                        rdfs:subClassOf op:InteractionFormula ;
                        rdfs:comment "Class to represent constant value mathematical formulas"@en ;
                        rdfs:label "Constant Value Formula"@en .


###  http://bimerr.iot.linkeddata.es/def/occupancy-profile#CustomProbabilityModel
op:CustomProbabilityModel rdf:type owl:Class ;
                          rdfs:subClassOf op:MovementModel ,
                                          [ rdf:type owl:Restriction ;
                                            owl:onProperty op:probability ;
                                            owl:someValuesFrom xsd:float
                                          ] ,
                                          [ rdf:type owl:Restriction ;
                                            owl:onProperty op:typicalTime ;
                                            owl:cardinality "1"^^xsd:nonNegativeInteger
                                          ] ;
                          rdfs:comment "Class to represent instances of custom probabilistic models."@en ;
                          rdfs:label "Custom probability model"@en .


###  http://bimerr.iot.linkeddata.es/def/occupancy-profile#Driver
op:Driver rdf:type owl:Class ;
          rdfs:comment "A Driver represents the environmental factor from the outside world that stimulate occupants in their inside world to fulfill a physical, physiological or psychological need."@en ;
          rdfs:label "Driver"@en .


###  http://bimerr.iot.linkeddata.es/def/occupancy-profile#DriverSet
op:DriverSet rdf:type owl:Class ;
             rdfs:subClassOf [ rdf:type owl:Restriction ;
                               owl:onProperty op:composedOf ;
                               owl:someValuesFrom op:Driver
                             ] ;
             rdfs:comment "Set of drivers that could be causing a behavior at a specific time."@en ;
             rdfs:label "Driver set"@en .


###  http://bimerr.iot.linkeddata.es/def/occupancy-profile#Environment
op:Environment rdf:type owl:Class ;
               rdfs:subClassOf op:Driver ,
                               [ rdf:type owl:Restriction ;
                                 owl:onProperty op:hasEnvironmentalParameter ;
                                 owl:someValuesFrom op:EnvironmentalParameter
                               ] ;
               rdfs:comment "Driver related to the environmental conditions that could be causing a behavior."@en ;
               rdfs:label "Environment"@en .


###  http://bimerr.iot.linkeddata.es/def/occupancy-profile#EnvironmentalParameter
op:EnvironmentalParameter rdf:type owl:Class ;
                          rdfs:subClassOf <https://w3id.org/saref#Property> ,
                                          [ rdf:type owl:Restriction ;
                                            owl:onProperty op:hasUnitOfMeasure ;
                                            owl:someValuesFrom <https://w3id.org/saref#UnitOfMeasure>
                                          ] ,
                                          [ rdf:type owl:Restriction ;
                                            owl:onProperty op:identifier ;
                                            owl:someValuesFrom xsd:string
                                          ] ;
                          rdfs:comment "Class that represent a physical variable of the environment where the driver occurs. It could represent variables that impact directly on the comfort levels of the occupant."@en ;
                          rdfs:label "Environmental parameter"@en .


###  http://bimerr.iot.linkeddata.es/def/occupancy-profile#Equipment
op:Equipment rdf:type owl:Class ;
             rdfs:subClassOf <https://w3id.org/saref#Device> ;
             rdfs:comment "Class to represent electrical equipments occupants interact with but do not have influence over indoor thermal conditions. These systems contribute to the energy bugdet estimation."@en ;
             rdfs:label "Equipment"@en .


###  http://bimerr.iot.linkeddata.es/def/occupancy-profile#Event
op:Event rdf:type owl:Class ;
         rdfs:subClassOf op:Driver ;
         rdfs:comment "Driver related to events that could be causing a behavior."@en ;
         rdfs:label "Event"@en .


###  http://bimerr.iot.linkeddata.es/def/occupancy-profile#Habit
op:Habit rdf:type owl:Class ;
         rdfs:subClassOf op:Driver ;
         rdfs:comment "Driver related to habits that could be causing a behavior."@en ;
         rdfs:label "Habit"@en .


###  http://bimerr.iot.linkeddata.es/def/occupancy-profile#IAQNeed
op:IAQNeed rdf:type owl:Class ;
           rdfs:subClassOf op:PhysicalNeed ;
           rdfs:comment "Range of parameter values where occupants do not feel indoor air quality discomfort and therefore, they don't carry out any actions."@en ;
           rdfs:label "IAQ Need"@en .


###  http://bimerr.iot.linkeddata.es/def/occupancy-profile#Inaction
op:Inaction rdf:type owl:Class .


###  http://bimerr.iot.linkeddata.es/def/occupancy-profile#Interaction
op:Interaction rdf:type owl:Class ;
               rdfs:subClassOf op:Action ,
                               [ rdf:type owl:Restriction ;
                                 owl:onProperty op:describedByFormula ;
                                 owl:someValuesFrom op:InteractionFormula
                               ] ,
                               [ rdf:type owl:Restriction ;
                                 owl:onProperty op:interactsOver ;
                                 owl:someValuesFrom s4bldg:BuildingObject
                               ] ,
                               [ rdf:type owl:Restriction ;
                                 owl:onProperty op:controlValue ;
                                 owl:someValuesFrom xsd:float
                               ] ;
               rdfs:comment "The Interaction class represent the interactions of occupants with systems within a space to recover their comfort."@en ;
               rdfs:label "Interaction"@en .


###  http://bimerr.iot.linkeddata.es/def/occupancy-profile#InteractionConcept
op:InteractionConcept rdf:type owl:Class ;
                      rdfs:subClassOf <http://www.w3.org/2004/02/skos/core#Concept> ;
                      rdfs:comment "Types of interactions between occupants and systems."@en ;
                      rdfs:label "Interaction concept"@en .


###  http://bimerr.iot.linkeddata.es/def/occupancy-profile#InteractionFormula
op:InteractionFormula rdf:type owl:Class ;
                      rdfs:subClassOf [ rdf:type owl:Restriction ;
                                        owl:onProperty op:hasCoefficient ;
                                        owl:someValuesFrom op:Coefficient
                                      ] ,
                                      [ rdf:type owl:Restriction ;
                                        owl:onProperty op:hasIndependentVariable ;
                                        owl:someValuesFrom op:EnvironmentalParameter
                                      ] ;
                      rdfs:comment "Formula to model the probability of interaction between ocupant and system."@en ;
                      rdfs:label "Interaction Formula"@en .


###  http://bimerr.iot.linkeddata.es/def/occupancy-profile#InteractionScheme
op:InteractionScheme rdf:type owl:Class ;
                     rdfs:subClassOf <http://www.w3.org/2004/02/skos/core#ConceptScheme> ;
                     rdfs:comment "An aggregation of SKOS concepts regarding the interaction type between occupants and space systems"@en ;
                     rdfs:label "Interaction scheme"@en .


###  http://bimerr.iot.linkeddata.es/def/occupancy-profile#LightingDevice
op:LightingDevice rdf:type owl:Class ;
                  rdfs:subClassOf <https://w3id.org/saref#Device> ;
                  rdfs:comment "A devide used for illumination."@en ;
                  rdfs:label "Lighting device"@en .


###  http://bimerr.iot.linkeddata.es/def/occupancy-profile#LinearFormula
op:LinearFormula rdf:type owl:Class ;
                 rdfs:subClassOf op:InteractionFormula ;
                 rdfs:comment "Class to represent linear mathematical formulas"@en ;
                 rdfs:label "Linear Formula"@en .


###  http://bimerr.iot.linkeddata.es/def/occupancy-profile#LogitFormula
op:LogitFormula rdf:type owl:Class ;
                rdfs:subClassOf op:InteractionFormula ;
                rdfs:comment "Class to represent logit mathematical formulas."@en ;
                rdfs:label "Logit Formula"@en .


###  http://bimerr.iot.linkeddata.es/def/occupancy-profile#MarkovChainModel
op:MarkovChainModel rdf:type owl:Class ;
                    rdfs:subClassOf op:MovementModel ,
                                    [ rdf:type owl:Restriction ;
                                      owl:onProperty op:earlyOccurTime ;
                                      owl:someValuesFrom xsd:time
                                    ] ,
                                    [ rdf:type owl:Restriction ;
                                      owl:onProperty op:typicalTime ;
                                      owl:someValuesFrom xsd:time
                                    ] ;
                    rdfs:comment "Class to represent instances of Markov chain models."@en ;
                    rdfs:label "Markov chain model"@en .


###  http://bimerr.iot.linkeddata.es/def/occupancy-profile#Meeting
op:Meeting rdf:type owl:Class ;
           rdfs:subClassOf [ rdf:type owl:Restriction ;
                             owl:onProperty op:duration ;
                             owl:someValuesFrom xsd:duration
                           ] ,
                           [ rdf:type owl:Restriction ;
                             owl:onProperty op:endTime ;
                             owl:someValuesFrom xsd:dateTime
                           ] ,
                           [ rdf:type owl:Restriction ;
                             owl:onProperty op:probability ;
                             owl:someValuesFrom xsd:float
                           ] ,
                           [ rdf:type owl:Restriction ;
                             owl:onProperty op:startTime ;
                             owl:someValuesFrom xsd:dateTime
                           ] ;
           rdfs:comment "Class to represent a meeting inside a communal space."@en ;
           rdfs:label "Meeting"@en .


###  http://bimerr.iot.linkeddata.es/def/occupancy-profile#Movement
op:Movement rdf:type owl:Class ;
            rdfs:subClassOf op:Action ;
            rdfs:comment "The Movement class is used to represent the occupant's movements inside or between spaces."@en ;
            rdfs:label "Movement"@en .


###  http://bimerr.iot.linkeddata.es/def/occupancy-profile#MovementModel
op:MovementModel rdf:type owl:Class ;
                 rdfs:comment "Probabilistic model to define occupant movements inside and between spaces."@en ;
                 rdfs:label "Movement Model"@en .


###  http://bimerr.iot.linkeddata.es/def/occupancy-profile#Need
op:Need rdf:type owl:Class ;
        rdfs:comment "Needs represent the physical and non-physical requirements of the occupant's inside world that must be met in order to ensure the satisfaction of the occupant with their environment."@en ;
        rdfs:label "Need"@en .


###  http://bimerr.iot.linkeddata.es/def/occupancy-profile#NonPhysicalNeed
op:NonPhysicalNeed rdf:type owl:Class ;
                   rdfs:subClassOf op:Need ;
                   owl:disjointWith op:PhysicalNeed ;
                   rdfs:comment "Non physical comfort needs (e.g. privacy, status, etc) that could influence a behavior."@en ;
                   rdfs:label "Non Physical Need"@en .


###  http://bimerr.iot.linkeddata.es/def/occupancy-profile#NormalProbabilityModel
op:NormalProbabilityModel rdf:type owl:Class ;
                          rdfs:subClassOf op:MovementModel ,
                                          [ rdf:type owl:Restriction ;
                                            owl:onProperty op:earlyOccurTime ;
                                            owl:someValuesFrom xsd:time
                                          ] ,
                                          [ rdf:type owl:Restriction ;
                                            owl:onProperty op:typicalTime ;
                                            owl:someValuesFrom xsd:time
                                          ] ;
                          rdfs:comment "Class to represent instances of Normal probabilistic models."@en ;
                          rdfs:label "Normal probability model"@en .


###  http://bimerr.iot.linkeddata.es/def/occupancy-profile#Occupant
op:Occupant rdf:type owl:Class ;
            rdfs:subClassOf foaf:Person ,
                            [ rdf:type owl:Restriction ;
                              owl:onProperty op:hasBehavior ;
                              owl:someValuesFrom op:Behavior
                            ] ,
                            [ rdf:type owl:Restriction ;
                              owl:onProperty op:identifier ;
                              owl:someValuesFrom xsd:string
                            ] ,
                            [ rdf:type owl:Restriction ;
                              owl:onProperty op:occupantAge ;
                              owl:allValuesFrom xsd:integer
                            ] ,
                            [ rdf:type owl:Restriction ;
                              owl:onProperty op:occupantGender ;
                              owl:allValuesFrom xsd:string
                            ] ,
                            [ rdf:type owl:Restriction ;
                              owl:onProperty op:occupantJobtype ;
                              owl:allValuesFrom xsd:string
                            ] ,
                            [ rdf:type owl:Restriction ;
                              owl:onProperty op:occupantLifestyle ;
                              owl:allValuesFrom xsd:string
                            ] ;
            rdfs:comment "Occupants or residents of a building."@en ;
            rdfs:label "Occupant"@en .


###  http://bimerr.iot.linkeddata.es/def/occupancy-profile#OperationalModeConcept
op:OperationalModeConcept rdf:type owl:Class ;
                          rdfs:subClassOf <http://www.w3.org/2004/02/skos/core#Concept> ;
                          rdfs:comment "Types of operational modes for space systems."@en ;
                          rdfs:label "Operational mode concept"@en .


###  http://bimerr.iot.linkeddata.es/def/occupancy-profile#OperationalModeConceptScheme
op:OperationalModeConceptScheme rdf:type owl:Class ;
                                rdfs:subClassOf <http://www.w3.org/2004/02/skos/core#ConceptScheme> ;
                                rdfs:comment "An aggregation of SKOS concepts regarding the operational mode of space systems."@en ;
                                rdfs:label "Operational mode scheme"@en .


###  http://bimerr.iot.linkeddata.es/def/occupancy-profile#ParameterRange
op:ParameterRange rdf:type owl:Class ;
                  rdfs:subClassOf [ rdf:type owl:Restriction ;
                                    owl:onProperty op:describesParameter ;
                                    owl:someValuesFrom op:EnvironmentalParameter
                                  ] ,
                                  [ rdf:type owl:Restriction ;
                                    owl:onProperty op:maxRangeValue ;
                                    owl:someValuesFrom xsd:float
                                  ] ,
                                  [ rdf:type owl:Restriction ;
                                    owl:onProperty op:minRangeValue ;
                                    owl:someValuesFrom xsd:float
                                  ] ;
                  rdfs:comment "Class to represent the minimum and maximm comfort values with respect to an environmental parameter."@en ;
                  rdfs:label "Parameter Range"@en .


###  http://bimerr.iot.linkeddata.es/def/occupancy-profile#PhysicalNeed
op:PhysicalNeed rdf:type owl:Class ;
                rdfs:subClassOf op:Need ,
                                [ rdf:type owl:Restriction ;
                                  owl:onProperty op:definedByRange ;
                                  owl:someValuesFrom op:ParameterRange
                                ] ;
                rdfs:comment "Physical comfort need that could influence a behavior."@en ;
                rdfs:label "Physical Need"@en .


###  http://bimerr.iot.linkeddata.es/def/occupancy-profile#QuadraticFormula
op:QuadraticFormula rdf:type owl:Class ;
                    rdfs:subClassOf op:InteractionFormula ;
                    rdfs:comment "Class to represent quadratic mathematical formulas."@en ;
                    rdfs:label "Quadratic Formula"@en .


###  http://bimerr.iot.linkeddata.es/def/occupancy-profile#RandomMovement
op:RandomMovement rdf:type owl:Class ;
                  rdfs:subClassOf op:Movement ;
                  rdfs:comment "Type of occupant movements inside a building or space."@en ;
                  rdfs:label "Random movement"@en .


###  http://bimerr.iot.linkeddata.es/def/occupancy-profile#Report
op:Report rdf:type owl:Class ;
          rdfs:subClassOf op:Action ;
          rdfs:comment "The Report class indicates that an occupant seeks assistance or files a complaint about their personal discomfort, but does not take direct action to satisfy their needs."@en ;
          rdfs:label "Report"@en .


###  http://bimerr.iot.linkeddata.es/def/occupancy-profile#Season
op:Season rdf:type owl:Class ;
          rdfs:subClassOf [ rdf:type owl:Restriction ;
                            owl:onProperty op:endSeason ;
                            owl:someValuesFrom xsd:gMonthDay
                          ] ,
                          [ rdf:type owl:Restriction ;
                            owl:onProperty op:startSeason ;
                            owl:someValuesFrom xsd:gMonthDay
                          ] ;
          rdfs:comment "Season of the year."@en ;
          rdfs:label "Season"@en .


###  http://bimerr.iot.linkeddata.es/def/occupancy-profile#SpaceOccupancy
op:SpaceOccupancy rdf:type owl:Class ;
                  rdfs:subClassOf op:RandomMovement ,
                                  [ rdf:type owl:Restriction ;
                                    owl:onProperty op:relatedToSpace ;
                                    owl:someValuesFrom building:Space
                                  ] ,
                                  [ rdf:type owl:Restriction ;
                                    owl:onProperty op:duration ;
                                    owl:someValuesFrom xsd:duration
                                  ] ,
                                  [ rdf:type owl:Restriction ;
                                    owl:onProperty op:percentTimePresence ;
                                    owl:someValuesFrom xsd:float
                                  ] ;
                  rdfs:comment "Occupancy percentage of staying in a specific space category in a building."@en ;
                  rdfs:label "Space occupancy"@en .


###  http://bimerr.iot.linkeddata.es/def/occupancy-profile#Spatial
op:Spatial rdf:type owl:Class ;
           rdfs:subClassOf op:Driver ,
                           [ rdf:type owl:Restriction ;
                             owl:onProperty op:detailedBy ;
                             owl:someValuesFrom building:Space
                           ] ;
           rdfs:comment "Driver related to spatial conditions that could be causing a behavior."@en ;
           rdfs:label "Spatial"@en .


###  http://bimerr.iot.linkeddata.es/def/occupancy-profile#StatusTransition
op:StatusTransition rdf:type owl:Class ;
                    rdfs:subClassOf op:Movement ,
                                    [ rdf:type owl:Restriction ;
                                      owl:onProperty op:hasTransitionType ;
                                      owl:someValuesFrom op:StatusTransitionTypeConcept
                                    ] ,
                                    [ rdf:type owl:Restriction ;
                                      owl:onProperty op:specifiedBy ;
                                      owl:someValuesFrom op:MovementModel
                                    ] ,
                                    [ rdf:type owl:Restriction ;
                                      owl:onProperty op:typicalDuration ;
                                      owl:someValuesFrom xsd:duration
                                    ] ;
                    rdfs:comment "Type of movements to represent transition events between spaces."@en ;
                    rdfs:label "Status transition"@en .


###  http://bimerr.iot.linkeddata.es/def/occupancy-profile#StatusTransitionScheme
op:StatusTransitionScheme rdf:type owl:Class ;
                          rdfs:subClassOf <http://www.w3.org/2004/02/skos/core#ConceptScheme> ;
                          rdfs:comment "An aggregation of SKOS concepts regarding the status transition type of movements between spaces."@en ;
                          rdfs:label "Status transition scheme"@en .


###  http://bimerr.iot.linkeddata.es/def/occupancy-profile#StatusTransitionTypeConcept
op:StatusTransitionTypeConcept rdf:type owl:Class ;
                               rdfs:subClassOf <http://www.w3.org/2004/02/skos/core#Concept> ;
                               rdfs:comment "One time event involving occupancy status transition in building level."@en ;
                               rdfs:label "Status transition type concept"@en .


###  http://bimerr.iot.linkeddata.es/def/occupancy-profile#ThermalNeed
op:ThermalNeed rdf:type owl:Class ;
               rdfs:subClassOf op:PhysicalNeed ;
               rdfs:comment "Range of parameter values where occupants do not feel thermal discomfort and therefore, they don't carry out any actions."@en ;
               rdfs:label "Thermal Need"@en .


###  http://bimerr.iot.linkeddata.es/def/occupancy-profile#Thermostat
op:Thermostat rdf:type owl:Class ;
              rdfs:subClassOf s4bldg:UnitaryControlElement ;
              rdfs:comment "A thermostat is a component which senses the temperature of a physical space and performs actions so that the space temperature is maintained near a desired setpoint. (Definition adapted from Wikipedia)"@en ;
              rdfs:label "Thermostat"@en .


###  http://bimerr.iot.linkeddata.es/def/occupancy-profile#Time
op:Time rdf:type owl:Class ;
        rdfs:subClassOf op:Driver ,
                        [ rdf:type owl:Restriction ;
                          owl:onProperty op:hasDayOfWeek ;
                          owl:allValuesFrom time:DayOfWeek
                        ] ,
                        [ rdf:type owl:Restriction ;
                          owl:onProperty op:hasSeason ;
                          owl:allValuesFrom op:Season
                        ] ,
                        [ rdf:type owl:Restriction ;
                          owl:onProperty op:hasTimeOfDay ;
                          owl:allValuesFrom op:TimeOfDay
                        ] ,
                        [ rdf:type owl:Restriction ;
                          owl:onProperty op:onHolidays ;
                          owl:allValuesFrom xsd:date
                        ] ;
        rdfs:comment "Driver related to time conditions that could be causing a behavior. It also describes the time when another type of driver occur."@en ;
        rdfs:label "Time"@en .


###  http://bimerr.iot.linkeddata.es/def/occupancy-profile#TimeOfDay
op:TimeOfDay rdf:type owl:Class ;
             rdfs:subClassOf [ rdf:type owl:Restriction ;
                               owl:onProperty op:endTime ;
                               owl:someValuesFrom xsd:time
                             ] ,
                             [ rdf:type owl:Restriction ;
                               owl:onProperty op:startTime ;
                               owl:someValuesFrom xsd:time
                             ] ;
             rdfs:comment "Relative time of day."@en ;
             rdfs:label "Time Of Day"@en .


###  http://bimerr.iot.linkeddata.es/def/occupancy-profile#VisualNeed
op:VisualNeed rdf:type owl:Class ;
              rdfs:subClassOf op:PhysicalNeed ;
              rdfs:comment "Range of parameter values where occupants do not feel visual discomfort and therefore, they don't carry out any actions."@en ;
              rdfs:label "Visual Need"@en .


###  http://bimerr.iot.linkeddata.es/def/occupancy-profile#WeibullFormula
op:WeibullFormula rdf:type owl:Class ;
                  rdfs:subClassOf op:InteractionFormula ;
                  rdfs:comment "Class to represent weibull mathematical formulas."@en ;
                  rdfs:label "Weibull Formula"@en .


###  http://bimerr.iot.linkeddata.es/def/occupancy-profile#Window
op:Window rdf:type owl:Class ;
          rdfs:subClassOf s4bldg:BuildingObject ;
          rdfs:comment "A window is an opening in a wall, door, roof or vehicle that allows the passage of light, sound, and sometimes air. (Definition taken from Wikipedia)"@en ;
          rdfs:label "Window"@en .


###  http://www.w3.org/2004/02/skos/core#Concept
<http://www.w3.org/2004/02/skos/core#Concept> rdf:type owl:Class ;
                                              rdfs:subClassOf [ rdf:type owl:Restriction ;
                                                                owl:onProperty <http://www.w3.org/2004/02/skos/core#broader> ;
                                                                owl:someValuesFrom <http://www.w3.org/2004/02/skos/core#Concept>
                                                              ] ,
                                                              [ rdf:type owl:Restriction ;
                                                                owl:onProperty <http://www.w3.org/2004/02/skos/core#inScheme> ;
                                                                owl:someValuesFrom <http://www.w3.org/2004/02/skos/core#ConceptScheme>
                                                              ] ,
                                                              [ rdf:type owl:Restriction ;
                                                                owl:onProperty <http://www.w3.org/2004/02/skos/core#narrower> ;
                                                                owl:someValuesFrom <http://www.w3.org/2004/02/skos/core#Concept>
                                                              ] ;
                                              rdfs:comment """The class skos:Concept is the class of SKOS concepts. A SKOS concept can be viewed as an idea or notion; a unit of thought. However, what constitutes a unit of thought is subjective, and this definition is meant to be suggestive, rather than restrictive.

The notion of a SKOS concept is useful when describing the conceptual or intellectual structure of a knowledge organization system, and when referring to specific ideas or meanings established within a KOS.

Note that, because SKOS is designed to be a vehicle for representing semi-formal KOS, such as thesauri and classification schemes, a certain amount of flexibility has been built in to the formal definition of this class."""@en ;
                                              rdfs:label "Concept"@en .


###  http://www.w3.org/2004/02/skos/core#ConceptScheme
<http://www.w3.org/2004/02/skos/core#ConceptScheme> rdf:type owl:Class ;
                                                    rdfs:comment """A SKOS concept scheme can be viewed as an aggregation of one or more SKOS concepts. Semantic relationships (links) between those concepts may also be viewed as part of a concept scheme. This definition is, however, meant to be suggestive rather than restrictive, and there is some flexibility in the formal data model stated below.

The notion of a concept scheme is useful when dealing with data from an unknown source, and when dealing with data that describes two or more different knowledge organization systems."""@en ;
                                                    rdfs:label "Concept Scheme"@en .


###  http://www.w3.org/2006/time#DayOfWeek
time:DayOfWeek rdf:type owl:Class ;
               rdfs:comment "The day of the week."@en ;
               rdfs:label "Day of week"@en .


###  http://xmlns.com/foaf/0.1#Person
foaf:Person rdf:type owl:Class ;
            rdfs:comment "The Person class represents people. Something is a Person if it is a person. We don't nitpic about whether they're alive, dead, real, or imaginary. (Definition taken from FOAF)"@en ;
            rdfs:label "Person"@en .


###  https://w3id.org/def/saref4building#BuildingObject
s4bldg:BuildingObject rdf:type owl:Class ;
                      rdfs:subClassOf s4bldg:PhysicalObject ;
                      rdfs:comment "An object in the building that can be controlled by devices, such as a door or a window that can be automatically opened or closed by an actuator. (Definition taken from SAREF 1.0)"@en ;
                      rdfs:label "Building object"@en .


###  https://w3id.org/def/saref4building#PhysicalObject
s4bldg:PhysicalObject rdf:type owl:Class ;
                      rdfs:subClassOf [ rdf:type owl:Restriction ;
                                        owl:onProperty op:hasOperationalMode ;
                                        owl:someValuesFrom op:OperationalModeConcept
                                      ] ;
                      rdfs:comment "Any Object that has a proper space region. (Definition extracted from DUL ontology)"@en ;
                      rdfs:label "Physical object"@en .


###  https://w3id.org/def/saref4building#ShadingDevice
s4bldg:ShadingDevice rdf:type owl:Class ;
                     rdfs:subClassOf <https://w3id.org/saref#Device> ;
                     rdfs:comment "Shading devices are purpose built devices to protect from the sunlight, from natural light, or screening them from view. Shading devices can form part of the facade or can be mounted inside the building, they can be fixed or operable. (Definition taken from S4BLDG ontology)"@en ;
                     rdfs:label "Shading device"@en .


###  https://w3id.org/def/saref4building#UnitaryControlElement
s4bldg:UnitaryControlElement rdf:type owl:Class ;
                             rdfs:subClassOf <https://w3id.org/saref#Device> ;
                             rdfs:comment "A unitary control element provides a housing for an aggregation of control or electrical distribution elements that, in combination, perform a singular (unitary) purpose. Each item in the aggregation may have its own geometric representation and location. (Definition taken from S4BLDG ontology)"@en ;
                             rdfs:label "Unitary control element"@en .


###  https://w3id.org/saref#Device
<https://w3id.org/saref#Device> rdf:type owl:Class ;
                                rdfs:subClassOf s4bldg:PhysicalObject ;
                                rdfs:comment "A tangible object designed to accomplish a particular task in households, common public buildings or offices. In order to accomplish this task, the device performs one or more functions. For example, a washing machine is designed to wash (task) and to accomplish this task it performs the start and stop function."@en ;
                                rdfs:label "Device"@en .


###  https://w3id.org/saref#HVAC
<https://w3id.org/saref#HVAC> rdf:type owl:Class ;
                              rdfs:subClassOf <https://w3id.org/saref#Device> ;
                              rdfs:comment "Heating, Ventilation and Air Conditioning (HVAC) device that provides indoor environmental comfort. A saref:HVAC is typically used to accomplish saref:Comfort."@en ;
                              rdfs:label "HVAC"@en .


###  https://w3id.org/saref#Property
<https://w3id.org/saref#Property> rdf:type owl:Class ;
                                  rdfs:comment "An aspect of an entity that can be observable by a sensor."@en ;
                                  rdfs:label "Property"@en .


###  https://w3id.org/saref#UnitOfMeasure
<https://w3id.org/saref#UnitOfMeasure> rdf:type owl:Class ;
                                       rdfs:comment "The unit of measure is a standard for measurement of a quantity, such as a Property. For example, Power is a property and Watt is a unit of power that represents a definite predetermined power: when we say 10 Watt, we actually mean 10 times the definite predetermined power called \"watt\". Our definition is based on the definition of unit of measure in the Ontology of units of Measure (OM). We propose here a list of some units of measure that are relevant for the purpose of the Smart Appliances ontology, but this list can be extended."@en ;
                                       rdfs:label "Unit of measure"@en .


#################################################################
#    Individuals
#################################################################

###  http://bimerr.iot.linkeddata.es/def/occupancy-profile#ASHRAEAdaptiveComfort
op:ASHRAEAdaptiveComfort rdf:type owl:NamedIndividual ,
                                  op:ThermalNeed .


###  http://bimerr.iot.linkeddata.es/def/occupancy-profile#ASHRAEComfortEnvelop
op:ASHRAEComfortEnvelop rdf:type owl:NamedIndividual ,
                                 op:ThermalNeed .


###  http://bimerr.iot.linkeddata.es/def/occupancy-profile#Adjustable
op:Adjustable rdf:type owl:NamedIndividual ,
                       op:OperationalModeConcept .


###  http://bimerr.iot.linkeddata.es/def/occupancy-profile#Afternoon
op:Afternoon rdf:type owl:NamedIndividual ,
                      op:TimeOfDay .


###  http://bimerr.iot.linkeddata.es/def/occupancy-profile#Arrival
op:Arrival rdf:type owl:NamedIndividual ,
                    op:StatusTransitionTypeConcept .


###  http://bimerr.iot.linkeddata.es/def/occupancy-profile#ContinuousControl
op:ContinuousControl rdf:type owl:NamedIndividual ,
                              op:OperationalModeConcept .


###  http://bimerr.iot.linkeddata.es/def/occupancy-profile#Day
op:Day rdf:type owl:NamedIndividual ,
                op:TimeOfDay .


###  http://bimerr.iot.linkeddata.es/def/occupancy-profile#DayLight
op:DayLight rdf:type owl:NamedIndividual ,
                     <https://w3id.org/saref#Property> .


###  http://bimerr.iot.linkeddata.es/def/occupancy-profile#Departure
op:Departure rdf:type owl:NamedIndividual ,
                      op:StatusTransitionTypeConcept .


###  http://bimerr.iot.linkeddata.es/def/occupancy-profile#EnteringRoom
op:EnteringRoom rdf:type owl:NamedIndividual ,
                         op:Event .


###  http://bimerr.iot.linkeddata.es/def/occupancy-profile#Evening
op:Evening rdf:type owl:NamedIndividual ,
                    op:TimeOfDay .


###  http://bimerr.iot.linkeddata.es/def/occupancy-profile#Fall
op:Fall rdf:type owl:NamedIndividual ,
                 op:Season .


###  http://bimerr.iot.linkeddata.es/def/occupancy-profile#Fixed
op:Fixed rdf:type owl:NamedIndividual ,
                  op:OperationalModeConcept .


###  http://bimerr.iot.linkeddata.es/def/occupancy-profile#Glare
op:Glare rdf:type owl:NamedIndividual ,
                  <https://w3id.org/saref#Property> .


###  http://bimerr.iot.linkeddata.es/def/occupancy-profile#ISOAdaptiveComfort
op:ISOAdaptiveComfort rdf:type owl:NamedIndividual ,
                               op:ThermalNeed .


###  http://bimerr.iot.linkeddata.es/def/occupancy-profile#Illuminance
op:Illuminance rdf:type owl:NamedIndividual ,
                        <https://w3id.org/saref#Property> .


###  http://bimerr.iot.linkeddata.es/def/occupancy-profile#Inaction
op:Inaction rdf:type owl:NamedIndividual ,
                     op:Inaction .


###  http://bimerr.iot.linkeddata.es/def/occupancy-profile#IndoorAirQuality
op:IndoorAirQuality rdf:type owl:NamedIndividual ,
                             <https://w3id.org/saref#Property> .


###  http://bimerr.iot.linkeddata.es/def/occupancy-profile#LeavingRoom
op:LeavingRoom rdf:type owl:NamedIndividual ,
                        op:Event .


###  http://bimerr.iot.linkeddata.es/def/occupancy-profile#Morning
op:Morning rdf:type owl:NamedIndividual ,
                    op:TimeOfDay .


###  http://bimerr.iot.linkeddata.es/def/occupancy-profile#Night
op:Night rdf:type owl:NamedIndividual ,
                  op:TimeOfDay .


###  http://bimerr.iot.linkeddata.es/def/occupancy-profile#Noise
op:Noise rdf:type owl:NamedIndividual ,
                  <https://w3id.org/saref#Property> .


###  http://bimerr.iot.linkeddata.es/def/occupancy-profile#Noon
op:Noon rdf:type owl:NamedIndividual ,
                 op:TimeOfDay .


###  http://bimerr.iot.linkeddata.es/def/occupancy-profile#OnOff
op:OnOff rdf:type owl:NamedIndividual ,
                  op:OperationalModeConcept .


###  http://bimerr.iot.linkeddata.es/def/occupancy-profile#Operable
op:Operable rdf:type owl:NamedIndividual ,
                     op:OperationalModeConcept .


###  http://bimerr.iot.linkeddata.es/def/occupancy-profile#Rain
op:Rain rdf:type owl:NamedIndividual ,
                 <https://w3id.org/saref#Property> .


###  http://bimerr.iot.linkeddata.es/def/occupancy-profile#RelativeHumidity
op:RelativeHumidity rdf:type owl:NamedIndividual ,
                             <https://w3id.org/saref#Property> .


###  http://bimerr.iot.linkeddata.es/def/occupancy-profile#SetToControlValue
op:SetToControlValue rdf:type owl:NamedIndividual ,
                              op:InteractionConcept .


###  http://bimerr.iot.linkeddata.es/def/occupancy-profile#ShortTermLeaving
op:ShortTermLeaving rdf:type owl:NamedIndividual ,
                             op:StatusTransitionTypeConcept .


###  http://bimerr.iot.linkeddata.es/def/occupancy-profile#ShortTermVisiting
op:ShortTermVisiting rdf:type owl:NamedIndividual ,
                              op:StatusTransitionTypeConcept .


###  http://bimerr.iot.linkeddata.es/def/occupancy-profile#SolarIrradiance
op:SolarIrradiance rdf:type owl:NamedIndividual ,
                            <https://w3id.org/saref#Property> .


###  http://bimerr.iot.linkeddata.es/def/occupancy-profile#Spring
op:Spring rdf:type owl:NamedIndividual ,
                   op:Season .


###  http://bimerr.iot.linkeddata.es/def/occupancy-profile#StayingInRoom
op:StayingInRoom rdf:type owl:NamedIndividual ,
                          op:Event .


###  http://bimerr.iot.linkeddata.es/def/occupancy-profile#Summer
op:Summer rdf:type owl:NamedIndividual ,
                   op:Season .


###  http://bimerr.iot.linkeddata.es/def/occupancy-profile#Temperature
op:Temperature rdf:type owl:NamedIndividual ,
                        <https://w3id.org/saref#Property> .


###  http://bimerr.iot.linkeddata.es/def/occupancy-profile#TurnOff
op:TurnOff rdf:type owl:NamedIndividual ,
                    op:InteractionConcept .


###  http://bimerr.iot.linkeddata.es/def/occupancy-profile#TurnOn
op:TurnOn rdf:type owl:NamedIndividual ,
                   op:InteractionConcept .


###  http://bimerr.iot.linkeddata.es/def/occupancy-profile#Winter
op:Winter rdf:type owl:NamedIndividual ,
                   op:Season .


###  http://bimerr.iot.linkeddata.es/def/occupancy-profile#ZoneOnOff
op:ZoneOnOff rdf:type owl:NamedIndividual ,
                      op:OperationalModeConcept .


###  http://www.w3.org/2006/time#Friday
time:Friday rdf:type owl:NamedIndividual ,
                     time:DayOfWeek .


###  http://www.w3.org/2006/time#Monday
time:Monday rdf:type owl:NamedIndividual ,
                     time:DayOfWeek .


###  http://www.w3.org/2006/time#Saturday
time:Saturday rdf:type owl:NamedIndividual ,
                       time:DayOfWeek .


###  http://www.w3.org/2006/time#Sunday
time:Sunday rdf:type owl:NamedIndividual ,
                     time:DayOfWeek .


###  http://www.w3.org/2006/time#Thursday
time:Thursday rdf:type owl:NamedIndividual ,
                       time:DayOfWeek .


###  http://www.w3.org/2006/time#Tuesday
time:Tuesday rdf:type owl:NamedIndividual ,
                      time:DayOfWeek .


###  http://www.w3.org/2006/time#Wednesday
time:Wednesday rdf:type owl:NamedIndividual ,
                        time:DayOfWeek .


#################################################################
#    Annotations
#################################################################

op:Inaction rdfs:label "Inaction"@en ;
            rdfs:comment "The Inaction class represents the decision of an occupant to not act and remain uncomfortable within a space."@en .


#################################################################
#    General axioms
#################################################################

[ rdf:type owl:AllDisjointClasses ;
  owl:members ( op:AccousticNeed
                op:IAQNeed
                op:ThermalNeed
                op:VisualNeed
              )
] .


[ rdf:type owl:AllDisjointClasses ;
  owl:members ( op:ConstantValueFormula
                op:LinearFormula
                op:LogitFormula
                op:QuadraticFormula
                op:WeibullFormula
              )
] .


[ rdf:type owl:AllDifferent ;
  owl:distinctMembers ( op:ASHRAEAdaptiveComfort
                        op:ASHRAEComfortEnvelop
                        op:ISOAdaptiveComfort
                      )
] .


###  Generated by the OWL API (version 4.5.9.2019-02-01T07:24:44Z) https://github.com/owlcs/owlapi
